\documentclass{article}
\usepackage{txfonts}
\usepackage{booktabs}
\usepackage{color}
\usepackage{bussproofs}

\begin{document}
\author{J. T. Klooster}
\title{Excersizes of Linear Logic}
\maketitle
\tableofcontents
\section{Seq calc vs N. D.}
\subsection{Give 2 variations of gentzen sequant calcules}

\begin{prooftree}
\AxiomC{$A \Rightarrow A$}
\AxiomC{$A \Rightarrow A$}
\AxiomC{$B \Rightarrow B$}
\AxiomC{$C \Rightarrow C$}
\RightLabel{$L\to$}
\BinaryInfC{$B\to C, B \Rightarrow C$}
\RightLabel{$L\to$}
\BinaryInfC{$\textcolor{red}{(A \to (B \to C))}, B, A \Rightarrow C$}
\RightLabel{$L\to$}
\BinaryInfC{$(A \to (B \to C)), \textcolor{red}{(A \to B)}, A,A \Rightarrow C$}
\RightLabel{$C$}
\UnaryInfC{$(A \to (B \to C)), (A \to B), A \Rightarrow C$}
\RightLabel{$R\to$}
\UnaryInfC{$(A \to (B \to C)), (A \to B) \Rightarrow  (A \to C)$}
\RightLabel{$R\to$}
\UnaryInfC{$(A \to (B \to C)) \Rightarrow  ((A \to B) \to (A \to C))$}
\RightLabel{$R\to$}
\UnaryInfC{$\Rightarrow (A \to (B \to C)) \to ((A \to B) \to (A \to C))$}
\end{prooftree}

\begin{prooftree}
\AxiomC{$A \Rightarrow A$}
\AxiomC{$A \Rightarrow A$}
\AxiomC{$B \Rightarrow B$}
\AxiomC{$C \Rightarrow C$}
\RightLabel{$L\to$}
\BinaryInfC{$B\to C, B \Rightarrow C$}
\RightLabel{$L\to$}
\BinaryInfC{$(B \to C)), \textcolor{red}{(A \to B)}, A \Rightarrow C$}
\RightLabel{$L\to$}
\BinaryInfC{$\textcolor{red}{(A \to (B \to C))}, (A \to B), A,A \Rightarrow C$}
\RightLabel{$C$}
\UnaryInfC{$(A \to (B \to C)), (A \to B), A \Rightarrow C$}
\RightLabel{$R\to$}
\UnaryInfC{$(A \to (B \to C)), (A \to B) \Rightarrow  (A \to C)$}
\RightLabel{$R\to$}
\UnaryInfC{$(A \to (B \to C)) \Rightarrow  ((A \to B) \to (A \to C))$}
\RightLabel{$R\to$}
\UnaryInfC{$\Rightarrow (A \to (B \to C)) \to ((A \to B) \to (A \to C))$}
\end{prooftree}
\subsection{Turn previous answers into natural deduction}

\begin{prooftree}
\AxiomC{$A \to(B \to C) \vdash A\to (B \to C)$}
\AxiomC{$A \vdash A$}
\RightLabel{$E\to$}
\BinaryInfC{$A \to (B \to C), A \vdash B \to C$}
\AxiomC{$A \to B \vdash A\to B$}
\AxiomC{$A \vdash A$}
\RightLabel{$E\to$}
\BinaryInfC{$A \to B, A\vdash B$}
\RightLabel{$E\to$}
\BinaryInfC{$A \to (B \to C), A \to B, A, A \vdash C$}
\RightLabel{C}
\UnaryInfC{$A \to (B \to C), A \to B, A \vdash C$}
\RightLabel{$I\to$}
\UnaryInfC{$A \to (B \to C), A \to B \vdash  (A \to C)$}
\RightLabel{$I\to$}
\UnaryInfC{$A \to (B \to C) \vdash  ((A \to B) \to (A \to C))$}
\RightLabel{$I\to$}
\UnaryInfC{$\vdash (A \to (B \to C)) \to ((A \to B) \to (A \to C))$}
\end{prooftree}

\section{Linear proofs}

\subsection{Two natural deduction proofs}
\begin{prooftree}
\AxiomC{$
	B \multimap C \vdash
	B \multimap C
$}
\AxiomC{$
	A \multimap B,
	\vdash
	A \multimap B,
$}
\AxiomC{$
	A \multimap A
	\vdash
	C
$}
\AxiomC{$
	A \multimap C,
	\vdash
	C
$}
\RightLabel{$E\multimap$}
\BinaryInfC{$
	A \multimap C,
	A \multimap A
	\vdash
	A
$}
\RightLabel{$E\multimap$}
\BinaryInfC{$
	A \multimap B,
	A \multimap C,
	A \multimap A
	\vdash
	B
$}
\RightLabel{$E\multimap$}
\BinaryInfC{$
	B \multimap C,
	A \multimap B,
	A \multimap C,
	A \multimap A
	\vdash
	C
$}
\RightLabel{$I\multimap$}
\UnaryInfC{$
	B \multimap C,
	A \multimap B,
	A \multimap C
	\vdash
	(A \multimap A) \multimap
	C
$}
\AxiomC{$
	A \vdash A
$}
\RightLabel{$I\multimap$}
\UnaryInfC{$
	\vdash
	A \multimap A
$}
\RightLabel{$E\multimap$}
\BinaryInfC{$
	B \multimap C,
	A \multimap B,
	A \multimap C
	\vdash
	C
$}
\RightLabel{$I\multimap$}
\LeftLabel{R}
\UnaryInfC{$
	B \multimap C,
	A \multimap B
	\vdash
	(A \multimap C) \multimap
	C
$}
\end{prooftree}
\begin{prooftree}

\AxiomC{$
	((A \multimap B) \multimap C) \multimap C \vdash
	((A \multimap B) \multimap C) \multimap C
$}
\AxiomC{$
	(A \multimap C) \multimap C,
	\vdash
	(A \multimap C) \multimap C,
$}
\AxiomC{$
	R
$}
\RightLabel{$E\multimap$}
\BinaryInfC{$
	(A \multimap C) \multimap C,
	B \multimap C,
	A \multimap B
	\vdash
	C
$}
\RightLabel{$I\multimap$}
\UnaryInfC{$
	(A \multimap C) \multimap C,
	B \multimap C,
	\vdash
	(A \multimap B) \multimap C
$}
\RightLabel{$E\multimap$}
\BinaryInfC{$
	(A \multimap C) \multimap C,
	B \multimap C,
	((A \multimap B) \multimap C) \multimap C \vdash
	C
	$
}
\RightLabel{$I\multimap$}
\UnaryInfC{$
	(A \multimap C) \multimap C,
	((A \multimap B) \multimap C) \multimap C \vdash
	(B \multimap C) \multimap C
	$
}
\end{prooftree}


\end{document}
