\documentclass{article}
\usepackage{txfonts}
\usepackage{booktabs}
\usepackage{color}
\usepackage{bussproofs}

\begin{document}
\author{J. T. Klooster}
\title{Excersizes of Linear Logic}
\maketitle
\tableofcontents
\section{Deriviations}
\begin{prooftree}
\RightLabel{Ax}
\AxiomC{}
\UnaryInfC{$
	((A \multimap B) \multimap B) \multimap B
	\vdash
	((A \multimap B) \multimap B) \multimap B
$}
\RightLabel{Ax}
\AxiomC{}
\UnaryInfC{$
	(A \multimap B) \multimap B
	\vdash
	(A \multimap B) \multimap B
$}
\RightLabel{Ax}
\AxiomC{}
\UnaryInfC{$
	A \multimap B
	\vdash
	A \multimap B
$}
\RightLabel{$E\multimap$}
\BinaryInfC{$
	(A \multimap B) \multimap B,
	A \multimap B
	\vdash
	B
$}
\RightLabel{$I\multimap$}
\UnaryInfC{$
	(A \multimap B) \multimap B
	\vdash
	(A \multimap B) \multimap B
$}
\RightLabel{$E\multimap$}
\BinaryInfC{$
	((A \multimap B) \multimap B) \multimap B,
	(A \multimap B) \multimap B
	\vdash
	B
$}
\RightLabel{$I\multimap$}
\UnaryInfC{$
	((A \multimap B) \multimap B) \multimap B
	\vdash
	((A \multimap B) \multimap B) \multimap B
$}
\RightLabel{$I\multimap$}
\UnaryInfC{$
	\vdash (((A \multimap B) \multimap B) \multimap B)
	\multimap
	(((A \multimap B) \multimap B) \multimap B)
$}
\end{prooftree}

\begin{prooftree}
\RightLabel{Ax}
\AxiomC{}
\UnaryInfC{$
	((A \multimap B) \multimap B) \multimap B
	\vdash
	((A \multimap B) \multimap B) \multimap B
$}
\RightLabel{Ax}
\AxiomC{}
\UnaryInfC{$
	(A \multimap B) \multimap B
	\vdash
	(A \multimap B) \multimap B
$}
\RightLabel{$E\multimap$}
\BinaryInfC{$
	((A \multimap B) \multimap B) \multimap B,
	(A \multimap B) \multimap B
	\vdash
	B
$}
\RightLabel{$I\multimap$}
\UnaryInfC{$
	((A \multimap B) \multimap B) \multimap B
	\vdash
	((A \multimap B) \multimap B) \multimap B
$}
\RightLabel{$I\multimap$}
\UnaryInfC{$
	\vdash (((A \multimap B) \multimap B) \multimap B)
	\multimap
	(((A \multimap B) \multimap B) \multimap B)
$}
\end{prooftree}

\section{Prove the ILL distributivity equivalance below}
To prove $A \otimes (B \oplus C) \vdash (A \otimes B)\oplus(A\times C)$ 
and $(A \otimes B)\oplus(A\otimes C) \vdash A \otimes (B \oplus C)$

\begin{prooftree}
\AxiomC{$
	\cdots
$}
\AxiomC{$
	\cdots
$}
\RightLabel{Ax}
\AxiomC{}
\UnaryInfC{$
	A \vdash A
$}
\RightLabel{Ax}
\AxiomC{}
\UnaryInfC{$
	B \vdash B
$}
\RightLabel{$I\otimes$}
\BinaryInfC{$
	A, B
	\vdash
	A\otimes B
$}
\RightLabel{$I\oplus$}
\UnaryInfC{$
	A, B
	\vdash
	(A \otimes B)\oplus(A\otimes C)
$}
\RightLabel{Ax}
\AxiomC{}
\UnaryInfC{$
	A \vdash A
$}
\RightLabel{Ax}
\AxiomC{}
\UnaryInfC{$
	C \vdash C
$}
\RightLabel{$I\otimes$}
\BinaryInfC{$
	A, C
	\vdash
	A\otimes C
$}
\RightLabel{$I\oplus$}
\UnaryInfC{$
	A, C
	\vdash
	(A \otimes B)\oplus(A\otimes C)
$}
\RightLabel{$E\oplus$}
\TrinaryInfC{$
	A, B \oplus C
	\vdash
	(A \otimes B)\oplus(A\otimes C)
$}
\RightLabel{$E\otimes$}
\BinaryInfC{$
	A \otimes (B \oplus C)
	\vdash
	(A \otimes B)\oplus(A\otimes C)
$}
\end{prooftree}

\begin{prooftree}
\AxiomC{$
$}
\RightLabel{$Ax$}
\UnaryInfC{$
	A \otimes B
	\vdash
	A \otimes B
$}
\RightLabel{$I\oplus$}
\UnaryInfC{$
	(A \otimes B)\oplus(A\otimes C)
	\vdash
	A \otimes B
$}
\AxiomC{$
$}
\RightLabel{$Ax$}
\UnaryInfC{$
	A \vdash A
$}
\AxiomC{$
$}
\RightLabel{$Ax$}
\UnaryInfC{$
	B \vdash B
$}
\RightLabel{$I\oplus$}
\UnaryInfC{$
	B \vdash
	B \oplus C
$}
\RightLabel{$I\otimes$}
\BinaryInfC{$
	A, B \vdash
	A \otimes (B \oplus C)
$}
\RightLabel{$E\otimes$}
\BinaryInfC{$
	(A \otimes B)\oplus(A\otimes C)
	\vdash
	A \otimes (B \oplus C)
$}
\end{prooftree}

\section{Prove these equivalences}

\begin{prooftree}
\AxiomC{$
	\cdots
$}
\AxiomC{$
$}
\RightLabel{$Ax$}
\UnaryInfC{$
	\langle A \rangle \vdash A
$}
\RightLabel{$I{!}$}
\UnaryInfC{$
	\langle A \rangle \vdash {!} A
$}
\AxiomC{$
$}
\RightLabel{$Ax$}
\UnaryInfC{$
	\langle {!}(A\& B) \rangle
	\vdash
	A \& B
$}
\RightLabel{$E\&$}
\UnaryInfC{$
	\langle {!}(A\& B) \rangle
	\vdash
	A
$}
\RightLabel{$I{!}$}
\UnaryInfC{$
	\langle {!}(A\& B) \rangle
	\vdash
	{!}A
$}
\RightLabel{$I\otimes$}
\BinaryInfC{$
	\langle {!}(A\& B) \rangle,
	\langle A\rangle
	\vdash
	{!}A \otimes {!}B
$}
\AxiomC{$
$}
\RightLabel{$Ax$}
\UnaryInfC{$
	\langle B \rangle \vdash B
$}
\RightLabel{$I{!}$}
\UnaryInfC{$
	\langle B \rangle \vdash {!} B
$}
\AxiomC{$
$}
\RightLabel{$Ax$}
\UnaryInfC{$
	\langle {!}(A\& B) \rangle
	\vdash
	A \& B
$}
\RightLabel{$E\&$}
\UnaryInfC{$
	\langle {!}(A\& B) \rangle
	\vdash
	A
$}
\RightLabel{$I{!}$}
\UnaryInfC{$
	\langle {!}(A\& B) \rangle
	\vdash
	{!}A
$}
\RightLabel{$I\otimes$}
\BinaryInfC{$
	\langle {!}(A\& B) \rangle,
	\langle B \rangle
	\vdash
	{!}A \otimes {!}B
$}
\RightLabel{$E\oplus$}
\TrinaryInfC{$
	\langle {!}(A\& B) \rangle
	\vdash
	{!}A \otimes {!}B
$}
\end{prooftree}
\begin{prooftree}
\AxiomC{$
$}
\RightLabel{$Ax$}
\UnaryInfC{$
	\langle {!}A \otimes {!}B\rangle
	\vdash
	A \otimes B
$}
\AxiomC{$
$}
\RightLabel{$Ax$}
\UnaryInfC{$
	\langle A \rangle
	\vdash
	A
$}
\RightLabel{$Weakening$}
\UnaryInfC{$
	\langle A \rangle , B
	\vdash
	A
$}
\AxiomC{$
$}
\RightLabel{$Ax$}
\UnaryInfC{$
	\langle B \rangle
	\vdash
	B
$}
\RightLabel{$Weakening$}
\UnaryInfC{$
	A, \langle B \rangle
	\vdash
	B
$}
\RightLabel{$I\&$}
\BinaryInfC{$
	\langle A \rangle , \langle B \rangle
	\vdash
	A\& B
$}
\RightLabel{$E\otimes$}
\BinaryInfC{$
	\langle {!}A \otimes {!}B\rangle
	\vdash
	A\& B
$}
\RightLabel{$I{!}$}
\UnaryInfC{$
	\langle {!}A \otimes {!}B\rangle
	\vdash
	{!}(A\& B)
$}
\end{prooftree}

\section{embedding IL into ILL}

\end{document}
