\documentclass{article}
\usepackage{txfonts}
\usepackage{booktabs}
\usepackage{color}
\usepackage{bussproofs}
\usepackage{graphicx}
\usepackage{pifont}
\newenvironment{scprooftree}[1]%
{\gdef\scalefactor{#1}\begin{center}\proofSkipAmount \leavevmode}%
{\scalebox{\scalefactor}{\DisplayProof}\proofSkipAmount \end{center} }

\begin{document}
\author{Jappie Klooster}
\title{Excersizes of Computational Logic}
\maketitle

\section{Commutative conversions}
\subsection{Missing parts}
\begin{scprooftree}{0.60}
\AxiomC{}
\RightLabel{Ax}
\UnaryInfC{$
	\langle d: (A \otimes B) \rangle
	\vdash
	d: A \otimes B
$}
\RightLabel{Ax}
\AxiomC{}
\UnaryInfC{$
	\langle f:B \rangle
	\vdash
	f:
	B
$}
\AxiomC{}
\RightLabel{Ax}
\UnaryInfC{$
	\langle g:A \rangle
	\vdash
	g:A
$}
\AxiomC{}
\RightLabel{Ax}
\UnaryInfC{$
	\langle x:A \multimap (B \multimap C) \rangle
	\vdash
	x:A \multimap (B \multimap C)
$}
\RightLabel{$E\multimap$}
\BinaryInfC{$
	\langle g: A \rangle,
	\langle x: A \multimap (B \multimap C) \rangle
	\vdash
	g\langle x\rangle:
	B \multimap C
$}
\RightLabel{$E\multimap$}
\BinaryInfC{$
	\langle g: A \rangle,
	\langle f: B \rangle,
	\langle x: A \multimap (B \multimap C) \rangle
	\vdash
	f\langle g\langle x\rangle\rangle:
	C
$}
\RightLabel{$E\otimes$}
\BinaryInfC{$
	\langle x: A \multimap (B \multimap C) \rangle,
	\langle d: (A \otimes B) \rangle
	\vdash
	$case $d$ of $ \langle g,f \rangle \to f\langle g\langle x\rangle\rangle:
	C
$}
\RightLabel{$I\multimap$}
\UnaryInfC{$
	\langle x: A \multimap (B \multimap C) \rangle
	\vdash
	\lambda \langle d \rangle {.} ($ case $d$ of $
	\langle g,f \rangle \to
	f\langle g\langle x\rangle\rangle):
	(A \otimes B) \multimap
	C
$}
\AxiomC{}
\RightLabel{Ax}
\UnaryInfC{$
	\langle c: A \rangle
	\vdash
	c:
	A
$}
\AxiomC{}
\RightLabel{Ax}
\UnaryInfC{$
	\langle b: B \rangle
	\vdash
	b:
	B
$}
\RightLabel{$I\otimes$}
\BinaryInfC{$
	\langle c:A \rangle,
	\langle b:B \rangle,
	\vdash
	\langle c,b \rangle :
	(A \otimes B)
$}
\RightLabel{$E\multimap$}
\BinaryInfC{$
	\langle c: A \rangle,
	\langle b: B \rangle,
	\langle x: A \multimap (B \multimap C) \rangle
	\vdash
	(\lambda \langle d \rangle {.} ($ case $d$ of $
	\langle g,f \rangle \to
	f\langle g\langle x\rangle\rangle)) \langle
	(\langle c,b \rangle )
	\rangle
	:
	C
$}
\end{scprooftree}
\subsection{Normal form}
The proof reductions I used was removing the unnescesaryy adding of
$A \otimes B$ via the $E \multimap$ operation.
This made the proof significantly smaller.

I found it by looking carefully at the proof and seeing that after the
$ E \otimes$ operation the proof is at the same stage as it was in the
beginning, so I just scrapped everything in between.

Now to justify this proof with help of the waldars paper. There are only
2 somewhat matching reductions applicble, the $E\otimes$ and the $E\multimap$
reductions. The problem with the $E\otimes$ is that its split into seperate
branches of the prooftree, so this would be impossible to apply without
getting rid first of the $E\multimap$. I end up proofing the tree before
even being able to apply the t part of the reduction.
(because adding $A \otimes B$ is unesesarry). So I guess I used the $E\multimap$
reduction of walders paper and that ends up being the following tree:
\begin{prooftree}
\RightLabel{Ax}
\AxiomC{}
\UnaryInfC{$
	\langle f:B \rangle
	\vdash
	f:
	B
$}
\AxiomC{}
\RightLabel{Ax}
\UnaryInfC{$
	\langle g:A \rangle
	\vdash
	g:A
$}
\AxiomC{}
\RightLabel{Ax}
\UnaryInfC{$
	\langle x:A \multimap (B \multimap C) \rangle
	\vdash
	x:A \multimap (B \multimap C)
$}
\RightLabel{$E\multimap$}
\BinaryInfC{$
	\langle g: A \rangle,
	\langle x: A \multimap (B \multimap C) \rangle
	\vdash
	g\langle x\rangle:
	B \multimap C
$}
\RightLabel{$E\multimap$}
\BinaryInfC{$
	\langle g: A \rangle,
	\langle f: B \rangle,
	\langle x: A \multimap (B \multimap C) \rangle
	\vdash
	f\langle g\langle x\rangle\rangle:
	C
$}
\end{prooftree}
\subsection{Term reductions}
\begin{prooftree}
\AxiomC{}
\UnaryInfC{$
	\langle c: A \rangle,
	\langle b: B \rangle,
	\langle x: A \multimap (B \multimap C) \rangle
	\vdash
	b\langle c\langle x\rangle\rangle
	:
	C
$}
\RightLabel{case $\langle t, u \rangle$ of $\langle x, y \rangle
	\to v \Rightarrow v[t/x, u/y]
$}
\UnaryInfC{$
	\langle c: A \rangle,
	\langle b: B \rangle,
	\langle x: A \multimap (B \multimap C) \rangle
	\vdash
	$ case $
	\langle c,b \rangle
	$ of $
	\langle g,f \rangle \to
	f\langle g\langle x\rangle\rangle
	:
	C
$}
\RightLabel{$
	(\lambda \langle x \rangle {.} u ) \langle t \rangle \Rightarrow u[t/x]
$}
\UnaryInfC{$
	\langle c: A \rangle,
	\langle b: B \rangle,
	\langle x: A \multimap (B \multimap C) \rangle
	\vdash
	(\lambda \langle d \rangle {.} ($ case $d$ of $
	\langle g,f \rangle \to
	f\langle g\langle x\rangle\rangle)) \langle
	\langle c,b \rangle
	\rangle
	:
	C
$}
\end{prooftree}

\section{Find ILL proof}
\begin{scprooftree}{0.9}
\AxiomC{}
\RightLabel{$
	Ax
$}
\UnaryInfC{$
	\langle y : {!}B \rangle
	\vdash
	y : {!}B
$}
\AxiomC{}
\RightLabel{$
	Ax
$}
\UnaryInfC{$
	\langle x : B \multimap (B \multimap A) \rangle,
	\vdash
	x : B \multimap (B \multimap A)
$}
\AxiomC{}
\RightLabel{$
	Ax
$}
\UnaryInfC{$
	[v:B]
	\vdash
	v : B
$}
\RightLabel{$
	E \multimap
$}
\BinaryInfC{$
	\langle x : B \multimap (B \multimap A) \rangle,
	[ v:B ]
	\vdash
	x \langle v \rangle
	: B \multimap A
$}
\AxiomC{}
\RightLabel{$
	Ax
$}
\UnaryInfC{$
	[ w:B] \vdash
	w:B
$}
\RightLabel{$
	E \multimap
$}
\BinaryInfC{$
	\langle x : B \multimap (B \multimap A) \rangle,
	[ w:B ],
	[ v:B ]
	\vdash
	x \langle v \rangle \langle w \rangle
	: A
$}
\RightLabel{$
	Cont
$}
\UnaryInfC{$
	\langle x : B \multimap (B \multimap A) \rangle,
	[ z:B ]
	\vdash
	x \langle z \rangle \langle z \rangle
	: A
$}
\RightLabel{$
	E{!}
$}
\BinaryInfC{$
	\langle x : B \multimap (B \multimap A) \rangle,
	\langle y : {!}B \rangle
	\vdash
	$case of $y$ of $!z \to x \langle z \rangle \langle z \rangle
	: A
$}
\RightLabel{$I \multimap$}
\UnaryInfC{$
	\langle x :B \multimap (B \multimap A) \rangle
	\vdash
	\lambda \langle y \rangle {.} 
	$case of $y$ of $!z \to x \langle z \rangle \langle z \rangle
	: {!}B \multimap A
$}
\RightLabel{$I \multimap$}
\UnaryInfC{$
	\vdash
	\lambda \langle x \rangle \lambda \langle y \rangle {.} 
	$case of $y$ of $!z \to x \langle z \rangle \langle z \rangle
	: (B \multimap (B \multimap A)) \multimap {!}B \multimap A
$}

\end{scprooftree}

\section{Translations}
I first made both proofs ILL because that is the most permisive system and
thus the easiest one.
This has the advantage that I already know the types.
After doing this I only had to change the operators and translate the program.

\subsection{Term one into ILL}
\begin{scprooftree}{0.7}
\AxiomC{}
\RightLabel{$
	Ax
$}
\UnaryInfC{$
	\langle x: ((A \multimap C) \multimap C) \multimap B \multimap D \rangle
	\vdash
	x: ((A \multimap C) \multimap C) \multimap B \multimap D
$}
\AxiomC{}
\RightLabel{$
	Ax
$}
\UnaryInfC{$
	\langle z:A \multimap C \rangle \vdash z:A \multimap C
$}
\AxiomC{}
\RightLabel{$
	Ax
$}
\UnaryInfC{$
	\langle w:A \rangle
	\vdash w: A
$}
\RightLabel{$
	E\multimap
$}
\BinaryInfC{$
	\langle z:A \multimap C \rangle,
	\langle w:A \rangle
	\vdash
	z \langle w \rangle
	:C
$}
\RightLabel{$
	Exchange
$}
\UnaryInfC{$
	\langle w:A \rangle,
	\langle z:A \multimap C \rangle
	\vdash
	z \langle w \rangle
	:C
$}
\RightLabel{$
	I\multimap
$}
\UnaryInfC{$
	\langle w:A \rangle
	\vdash
	\lambda \langle z \rangle
	{.}z \langle w \rangle
	: (A \multimap C) \multimap C
$}
\RightLabel{$
	E \multimap
$}
\BinaryInfC{$
	\langle x: ((A \multimap C) \multimap C) \multimap B \multimap D \rangle,
	\langle w:A \rangle
	\vdash
	x
	\langle
		\lambda \langle z \rangle
		{.}z \langle w \rangle
	\rangle
	: B \multimap D
$}
\AxiomC{}
\RightLabel{$
	Ax
$}
\UnaryInfC{$
	\langle y:B \rangle
	\vdash
	y:B
$}
\RightLabel{$
	E \multimap
$}
\BinaryInfC{$
	\langle x: ((A \multimap C) \multimap C) \multimap B \multimap D \rangle,
	\langle w:A \rangle,
	\langle y:B \rangle
	\vdash
	x
	\langle
		\lambda \langle z \rangle
		{.}z \langle w \rangle
	\rangle
	\langle y \rangle
	: D
$}
\RightLabel{$
	I \multimap
$}
\UnaryInfC{$
	\langle x: ((A \multimap C) \multimap C) \multimap B \multimap D \rangle,
	\langle w:A \rangle
	\vdash
	\lambda \langle y \rangle{.}x
	\langle
		\lambda \langle z \rangle
		{.}z \langle w \rangle
	\rangle
	\langle y \rangle
	: B \multimap D
$}
\RightLabel{$
	I \multimap
$}
\UnaryInfC{$
	\langle x: ((A \multimap C) \multimap C) \multimap B \multimap D \rangle
	\vdash
	\lambda \langle w \rangle \lambda \langle y \rangle{.}x
	\langle
		\lambda \langle z \rangle
		{.}z \langle w \rangle
	\rangle
	\langle y \rangle
	: A \multimap (B \multimap D)
$}
\end{scprooftree}

\subsection{Term one into grammar}
\begin{scprooftree}{0.7}
\AxiomC{}
\RightLabel{$
	Ax
$}
\UnaryInfC{$
	\langle x: (D / B) / ((A/ C)\setminus C) \rangle
	\vdash
	x: (D / B) / ((A/ C)\setminus C)
$}
\AxiomC{}
\RightLabel{$
	Ax
$}
\UnaryInfC{$
	\langle z:A/C \rangle
	\vdash
	z:A/C
$}
\AxiomC{}
\RightLabel{$
	Ax
$}
\UnaryInfC{$
	\langle w:A \rangle
	\vdash w: A
$}
\RightLabel{$
	E/
$}
\BinaryInfC{$
	\langle z:A/C \rangle,
	\langle w:A \rangle
	\vdash
	z \lhd w
	:C
$}
\RightLabel{$
	I\setminus
$}
\UnaryInfC{$
	\langle w:A \rangle
	\vdash
	\overleftarrow{\lambda} z{.}(z \lhd w )
	: (A / C)\setminus C
$}
\RightLabel{$
	E/
$}
\BinaryInfC{$
	\langle x: (D / B) / ((A/ C)\setminus C) \rangle,
	\langle w:A \rangle
	\vdash
	x
	\lhd
		( \overleftarrow{\lambda} z
			{.}(z \lhd w )
		)
	: D/B
$}
\AxiomC{}
\RightLabel{$
	Ax
$}
\UnaryInfC{$
	\langle y:B \rangle
	\vdash
	y:B
$}
\RightLabel{$
	E/
$}
\BinaryInfC{$
	\langle x: (D / B) / ((A/ C)\setminus C) \rangle,
	\langle w:A \rangle,
	\langle y:B \rangle
	\vdash
	(x
	\lhd
		( \overleftarrow{\lambda} z
			{.}(z \lhd w )
		)
	)
	\lhd y
	: D
$}
\RightLabel{$
	I /
$}
\UnaryInfC{$
	\langle x: (D / B) / ((A/ C)\setminus C) \rangle,
	\langle w:A \rangle
	\vdash
	\overrightarrow{\lambda} y{.}(
		(x
		\lhd
			( \overleftarrow{\lambda} z
				{.}(z \lhd w )
			)
		)
		\lhd y
	)
	: B/D
$}
\RightLabel{$
	I /
$}
\UnaryInfC{$
	\langle x: (D / B) / ((A/ C)\setminus C) \rangle
	\vdash
	\overrightarrow{\lambda} w {.}(
		\overrightarrow{\lambda} y{.}(
			(x
			\lhd
				( \overleftarrow{\lambda} z
					{.}(z \lhd w )
				)
			)
			\lhd y
		)
	)
	: A/(B/D)
$}
\end{scprooftree}

\subsection{Term two into ILL}
\begin{scprooftree}{0.8}
\AxiomC{}
\RightLabel{$
	Ax
$}
\UnaryInfC{$
	\langle w:(C \multimap D) \multimap A \rangle
	\vdash
	w:(C \multimap D) \multimap A
$}
\AxiomC {}
\RightLabel{$
	Ax
$}
\UnaryInfC{$
	\langle x:C \multimap (B \multimap D) \rangle
	\vdash
	x: C \multimap (B \multimap D)
$}
\AxiomC {}
\RightLabel{$
	Ax
$}
\UnaryInfC{$
	\langle z:C \rangle
	\vdash
	z:C
$}
\RightLabel{$
	E \multimap
$}
\BinaryInfC{$
	\langle x:C \multimap (B \multimap D) \rangle,
	\langle z:C \rangle,
	\vdash
	x \langle z \rangle
	: B \multimap D
$}
\AxiomC{}
\RightLabel{$
	Ax
$}
\UnaryInfC{$
	\langle y:B \rangle
	\vdash
	y:B
$}
\BinaryInfC{$
	\langle x:C \multimap (B \multimap D) \rangle,
	\langle z:C \rangle,
	\langle y:B \rangle
	\vdash
	x \langle z \rangle
	\langle y \rangle
	: D
$}
\RightLabel{$
	Exchange
$}
\UnaryInfC{$
	\langle x:C \multimap (B \multimap D) \rangle,
	\langle y:B \rangle,
	\langle z:C \rangle
	\vdash
		{.}x \langle z \rangle
	\langle y \rangle
	: D
$}
\RightLabel{$
	I \multimap
$}
\UnaryInfC{$
	\langle x:C \multimap (B \multimap D) \rangle,
	\langle y:B \rangle
	\vdash
		\lambda \langle z \rangle
		{.}x \langle z \rangle
	\langle y \rangle
	: C \multimap D
$}
\RightLabel{$
	E \multimap
$}
\BinaryInfC{$
	\langle w:(C \multimap D) \multimap A \rangle,
	\langle x:C \multimap (B \multimap D) \rangle,
	\langle y:B \rangle
	\vdash
	w
	\langle
		\lambda \langle z \rangle
		{.}x \langle z \rangle
	\langle y \rangle
	\rangle
	: A
$}
\RightLabel{$
	Exchange
$}
\UnaryInfC{$
	\langle x:C \multimap (B \multimap D) \rangle,
	\langle w:(C \multimap D) \multimap A \rangle,
	\langle y:B \rangle
	\vdash
	w
	\langle
		\lambda \langle z \rangle
		{.}x \langle z \rangle
	\langle y \rangle
	\rangle
	: A
$}
\RightLabel{$
	I \multimap
$}
\UnaryInfC{$
	\langle x:C \multimap (B \multimap D) \rangle,
	\langle w:(C \multimap D) \multimap A \rangle
	\vdash
	\lambda \langle y \rangle
	{.}w
	\langle
		\lambda \langle z \rangle
		{.}x \langle z \rangle
	\langle y \rangle
	\rangle
	: B \multimap A
$}
\RightLabel{$
	I \multimap
$}
\UnaryInfC{$
	\langle x:C \multimap (B \multimap D) \rangle
	\vdash
	\lambda \langle w \rangle \lambda \langle y \rangle
	{.}w
	\langle
		\lambda \langle z \rangle
		{.}x \langle z \rangle
	\langle y \rangle
	\rangle
	: ((C \multimap D) \multimap A) \multimap (B \multimap A)
$}
\end{scprooftree}

\subsection{Term two into grammar}
Term two can't be translated into grammar logic because the y can never find
the right position. It will always be introduced to early to either become
problematic for other terms later or it can't become an axiom itself.
\end{document}
